ocaml/fstar-lib/generated/FStar_Main.ml
@@ -288,6 +288,8 @@ let (lazy_chooser :
           FStar_Reflection_Embeddings.unfold_lazy_universe i
       | FStar_Syntax_Syntax.Lazy_universe_uvar ->
           FStar_Syntax_Util.exp_string "((universe_uvar))"
+      | FStar_Syntax_Syntax.Lazy_issue ->
+          FStar_Syntax_Util.exp_string "((issue))"
 let (setup_hooks : unit -> unit) =
   fun uu___ ->
     FStar_Errors.set_parse_warn_error FStar_Parser_ParseIt.parse_warn_error;
