src/syntax/FStar.Syntax.Embeddings.fst
@@ -887,7 +887,33 @@ let e_range =
         S.t_range
         Range.string_of_range
         (ET_app (PC.range_lid |> Ident.string_of_lid, []))
-        
+
+let e_issue =
+    let t_issue = 
+            S.fv_to_tm 
+                    (S.lid_as_fv PC.issue_lid
+                                 S.delta_constant
+                                 None)
+    in              
+    let em (i:FStar.Errors.issue) (rng:range) _shadow _norm : term = 
+        U.mk_lazy i t_issue Lazy_issue (Some rng)
+    in
+    let un (t0:term) (w:bool) _norm : option FStar.Errors.issue =
+        let t = unmeta_div_results t0 in
+        match t.n with
+        | Tm_lazy { lkind = Lazy_issue; blob } -> Some (Dyn.undyn blob)
+        | _ ->
+            if w then
+            Err.log_issue t0.pos (Err.Warning_NotEmbedded, (BU.format1 "Not an embedded issue: %s" (Print.term_to_string t0)));
+            None
+    in
+    mk_emb_full
+        em
+        un
+        t_issue
+        (fun i -> BU.format1 "%s" (FStar.Errors.format_issue i))
+        (ET_app (PC.issue_lid |> Ident.string_of_lid, []))
+    
 let e_vconfig =
     let em (vcfg:vconfig) (rng:Range.range) _shadow norm : term =
       (* The order is very important here, even if this is a record. *)
