src/syntax/FStar.Syntax.Syntax.fsti
@@ -378,6 +378,7 @@ and lazy_kind =
   | Lazy_embedding of emb_typ * Thunk.t term
   | Lazy_universe
   | Lazy_universe_uvar
+  | Lazy_issue
 and binding =
   | Binding_var      of bv
   | Binding_lid      of lident * (univ_names * typ)
